Bench.v
@@ -1,0 +1,31 @@
+
+Require Import ZArith.
+Require Import Coq.Strings.String.
+Require Import List. Import ListNotations.
+
+Set Warnings "-extraction-reserved-identifier".
+
+From QuickChick Require Import QuickChick.
+
+Require Import IFC.Rules.
+Require Import IFC.TestingCommon.
+Require Import IFC.Generation.
+Require Import IFC.Shrinking.
+Require Import IFC.SSNI.
+Require Import IFC.Reachability.
+Require Import IFC.SingleStateArb.
+
+Require Import IFC.SanityChecks.
+
+Require Import Mutate.
+
+Definition testMutantX_ p n : Checker :=
+  p (nth n (mutate_table default_table) default_table).
+
+Definition rSSNI_smart := propSSNI_smart exp_result_random.
+Definition fSSNI_smart := propSSNI_smart exp_result_fuzz.
+Definition rSSNI_naive := propSSNI_arb   exp_result_random.
+Definition fSSNI_naive := propSSNI_arb   exp_result_fuzz.
+
+QuickChick (testMutantX_ rSSNI_naive 0).
+FuzzChick (testMutantX_ 0).
